src/HOL/Auth/NS_Public_Bad.thy
@@ -11,38 +11,222 @@ From page 260 of
   Proc. Royal Soc. 426 (1989)
 *)
 
-NS_Public_Bad = Public + 
+theory NS_Public_Bad = Public:
 
-consts  ns_public  :: event list set
+consts  ns_public  :: "event list set"
 
 inductive ns_public
-  intrs 
+  intros 
          (*Initial trace is empty*)
-    Nil  "[]: ns_public"
+   Nil:  "[] \<in> ns_public"
 
          (*The spy MAY say anything he CAN say.  We do not expect him to
            invent new nonces here, but he can also use NS1.  Common to
            all similar protocols.*)
-    Fake "[| evs: ns_public;  X: synth (analz (spies evs)) |]
-          ==> Says Spy B X  # evs : ns_public"
+   Fake: "\<lbrakk>evs \<in> ns_public;  X \<in> synth (analz (spies evs))\<rbrakk>
+          \<Longrightarrow> Says Spy B X  # evs \<in> ns_public"
 
          (*Alice initiates a protocol run, sending a nonce to Bob*)
-    NS1  "[| evs1: ns_public;  Nonce NA ~: used evs1 |]
-          ==> Says A B (Crypt (pubK B) {|Nonce NA, Agent A|})
-                # evs1  :  ns_public"
+   NS1:  "\<lbrakk>evs1 \<in> ns_public;  Nonce NA \<notin> used evs1\<rbrakk>
+          \<Longrightarrow> Says A B (Crypt (pubK B) \<lbrace>Nonce NA, Agent A\<rbrace>)
+                # evs1  \<in>  ns_public"
 
          (*Bob responds to Alice's message with a further nonce*)
-    NS2  "[| evs2: ns_public;  Nonce NB ~: used evs2;
-             Says A' B (Crypt (pubK B) {|Nonce NA, Agent A|}) : set evs2 |]
-          ==> Says B A (Crypt (pubK A) {|Nonce NA, Nonce NB|})
-                # evs2  :  ns_public"
+   NS2:  "\<lbrakk>evs2 \<in> ns_public;  Nonce NB \<notin> used evs2;
+           Says A' B (Crypt (pubK B) \<lbrace>Nonce NA, Agent A\<rbrace>) \<in> set evs2\<rbrakk>
+          \<Longrightarrow> Says B A (Crypt (pubK A) \<lbrace>Nonce NA, Nonce NB\<rbrace>)
+                # evs2  \<in>  ns_public"
 
          (*Alice proves her existence by sending NB back to Bob.*)
-    NS3  "[| evs3: ns_public;
-             Says A  B (Crypt (pubK B) {|Nonce NA, Agent A|}) : set evs3;
-             Says B' A (Crypt (pubK A) {|Nonce NA, Nonce NB|}) : set evs3 |]
-          ==> Says A B (Crypt (pubK B) (Nonce NB)) # evs3 : ns_public"
+   NS3:  "\<lbrakk>evs3 \<in> ns_public;
+           Says A  B (Crypt (pubK B) \<lbrace>Nonce NA, Agent A\<rbrace>) \<in> set evs3;
+           Says B' A (Crypt (pubK A) \<lbrace>Nonce NA, Nonce NB\<rbrace>) \<in> set evs3\<rbrakk>
+          \<Longrightarrow> Says A B (Crypt (pubK B) (Nonce NB)) # evs3 \<in> ns_public"
 
-  (**Oops message??**)
+  (*No Oops message.  Should there be one?*)
+
+declare knows_Spy_partsEs [elim]
+declare analz_subset_parts [THEN subsetD, dest]
+declare Fake_parts_insert [THEN subsetD, dest]
+declare image_eq_UN [simp]  (*accelerates proofs involving nested images*)
+
+(*A "possibility property": there are traces that reach the end*)
+lemma "\<exists>NB. \<exists>evs \<in> ns_public. Says A B (Crypt (pubK B) (Nonce NB)) \<in> set evs"
+apply (intro exI bexI)
+apply (rule_tac [2] ns_public.Nil [THEN ns_public.NS1, THEN ns_public.NS2, 
+                                   THEN ns_public.NS3])
+by possibility
+
+
+(**** Inductive proofs about ns_public ****)
+
+(** Theorems of the form X \<notin> parts (spies evs) imply that NOBODY
+    sends messages containing X! **)
+
+(*Spy never sees another agent's private key! (unless it's bad at start)*)
+lemma Spy_see_priK [simp]: 
+      "evs \<in> ns_public \<Longrightarrow> (Key (priK A) \<in> parts (spies evs)) = (A \<in> bad)"
+by (erule ns_public.induct, auto)
+
+lemma Spy_analz_priK [simp]: 
+      "evs \<in> ns_public \<Longrightarrow> (Key (priK A) \<in> analz (spies evs)) = (A \<in> bad)"
+by auto
+
+
+(*** Authenticity properties obtained from NS2 ***)
+
+(*It is impossible to re-use a nonce in both NS1 and NS2, provided the nonce
+  is secret.  (Honest users generate fresh nonces.)*)
+lemma no_nonce_NS1_NS2 [rule_format]: 
+      "evs \<in> ns_public 
+       \<Longrightarrow> Crypt (pubK C) \<lbrace>NA', Nonce NA\<rbrace> \<in> parts (spies evs) \<longrightarrow>
+           Crypt (pubK B) \<lbrace>Nonce NA, Agent A\<rbrace> \<in> parts (spies evs) \<longrightarrow>  
+           Nonce NA \<in> analz (spies evs)"
+apply (erule ns_public.induct, simp_all)
+apply (blast intro: analz_insertI)+
+done
+
+
+(*Unicity for NS1: nonce NA identifies agents A and B*)
+lemma unique_NA: 
+     "\<lbrakk>Crypt(pubK B)  \<lbrace>Nonce NA, Agent A \<rbrace> \<in> parts(spies evs);  
+       Crypt(pubK B') \<lbrace>Nonce NA, Agent A'\<rbrace> \<in> parts(spies evs);  
+       Nonce NA \<notin> analz (spies evs); evs \<in> ns_public\<rbrakk>
+      \<Longrightarrow> A=A' \<and> B=B'"
+apply (erule rev_mp, erule rev_mp, erule rev_mp)   
+apply (erule ns_public.induct, simp_all)
+(*Fake, NS1*)
+apply (blast intro!: analz_insertI)+
+done
+
+
+(*Secrecy: Spy does not see the nonce sent in msg NS1 if A and B are secure
+  The major premise "Says A B ..." makes it a dest-rule, so we use
+  (erule rev_mp) rather than rule_format. *)
+theorem Spy_not_see_NA: 
+      "\<lbrakk>Says A B (Crypt(pubK B) \<lbrace>Nonce NA, Agent A\<rbrace>) \<in> set evs;
+        A \<notin> bad;  B \<notin> bad;  evs \<in> ns_public\<rbrakk>                     
+       \<Longrightarrow> Nonce NA \<notin> analz (spies evs)"
+apply (erule rev_mp)   
+apply (erule ns_public.induct, simp_all)
+apply spy_analz
+apply (blast dest: unique_NA intro: no_nonce_NS1_NS2)+
+done
+
+
+(*Authentication for A: if she receives message 2 and has used NA
+  to start a run, then B has sent message 2.*)
+lemma A_trusts_NS2_lemma [rule_format]: 
+   "\<lbrakk>A \<notin> bad;  B \<notin> bad;  evs \<in> ns_public\<rbrakk>                     
+    \<Longrightarrow> Crypt (pubK A) \<lbrace>Nonce NA, Nonce NB\<rbrace> \<in> parts (spies evs) \<longrightarrow>
+	Says A B (Crypt(pubK B) \<lbrace>Nonce NA, Agent A\<rbrace>) \<in> set evs \<longrightarrow>
+	Says B A (Crypt(pubK A) \<lbrace>Nonce NA, Nonce NB\<rbrace>) \<in> set evs"
+apply (erule ns_public.induct)
+apply (auto dest: Spy_not_see_NA unique_NA)
+done
+
+theorem A_trusts_NS2: 
+     "\<lbrakk>Says A  B (Crypt(pubK B) \<lbrace>Nonce NA, Agent A\<rbrace>) \<in> set evs;   
+       Says B' A (Crypt(pubK A) \<lbrace>Nonce NA, Nonce NB\<rbrace>) \<in> set evs;
+       A \<notin> bad;  B \<notin> bad;  evs \<in> ns_public\<rbrakk>                     
+      \<Longrightarrow> Says B A (Crypt(pubK A) \<lbrace>Nonce NA, Nonce NB\<rbrace>) \<in> set evs"
+by (blast intro: A_trusts_NS2_lemma)
+
+
+(*If the encrypted message appears then it originated with Alice in NS1*)
+lemma B_trusts_NS1 [rule_format]:
+     "evs \<in> ns_public                                         
+      \<Longrightarrow> Crypt (pubK B) \<lbrace>Nonce NA, Agent A\<rbrace> \<in> parts (spies evs) \<longrightarrow>
+	  Nonce NA \<notin> analz (spies evs) \<longrightarrow>
+	  Says A B (Crypt (pubK B) \<lbrace>Nonce NA, Agent A\<rbrace>) \<in> set evs"
+apply (erule ns_public.induct, simp_all)
+(*Fake*)
+apply (blast intro!: analz_insertI)
+done
+
+
+
+(*** Authenticity properties obtained from NS2 ***)
+
+(*Unicity for NS2: nonce NB identifies nonce NA and agent A
+  [proof closely follows that for unique_NA] *)
+lemma unique_NB [dest]: 
+     "\<lbrakk>Crypt(pubK A)  \<lbrace>Nonce NA, Nonce NB\<rbrace> \<in> parts(spies evs);
+       Crypt(pubK A') \<lbrace>Nonce NA', Nonce NB\<rbrace> \<in> parts(spies evs);
+       Nonce NB \<notin> analz (spies evs); evs \<in> ns_public\<rbrakk>
+     \<Longrightarrow> A=A' \<and> NA=NA'"
+apply (erule rev_mp, erule rev_mp, erule rev_mp)   
+apply (erule ns_public.induct, simp_all)
+(*Fake, NS2*)
+apply (blast intro!: analz_insertI)+
+done
+
+
+(*NB remains secret PROVIDED Alice never responds with round 3*)
+theorem Spy_not_see_NB [dest]:
+     "\<lbrakk>Says B A (Crypt (pubK A) \<lbrace>Nonce NA, Nonce NB\<rbrace>) \<in> set evs;   
+       \<forall>C. Says A C (Crypt (pubK C) (Nonce NB)) \<notin> set evs;       
+       A \<notin> bad;  B \<notin> bad;  evs \<in> ns_public\<rbrakk>                      
+     \<Longrightarrow> Nonce NB \<notin> analz (spies evs)"
+apply (erule rev_mp, erule rev_mp)
+apply (erule ns_public.induct, simp_all)
+apply spy_analz
+apply (simp_all add: all_conj_distrib) (*speeds up the next step*)
+apply (blast intro: no_nonce_NS1_NS2)+
+done
+
+
+(*Authentication for B: if he receives message 3 and has used NB
+  in message 2, then A has sent message 3--to somebody....*)
+
+lemma B_trusts_NS3_lemma [rule_format]:
+     "\<lbrakk>A \<notin> bad;  B \<notin> bad;  evs \<in> ns_public\<rbrakk>                    
+      \<Longrightarrow> Crypt (pubK B) (Nonce NB) \<in> parts (spies evs) \<longrightarrow>
+          Says B A  (Crypt (pubK A) \<lbrace>Nonce NA, Nonce NB\<rbrace>) \<in> set evs \<longrightarrow>
+          (\<exists>C. Says A C (Crypt (pubK C) (Nonce NB)) \<in> set evs)"
+apply (erule ns_public.induct, auto)
+by (blast intro: no_nonce_NS1_NS2)+
+
+theorem B_trusts_NS3:
+     "\<lbrakk>Says B A  (Crypt (pubK A) \<lbrace>Nonce NA, Nonce NB\<rbrace>) \<in> set evs;
+       Says A' B (Crypt (pubK B) (Nonce NB)) \<in> set evs;             
+       A \<notin> bad;  B \<notin> bad;  evs \<in> ns_public\<rbrakk>                    
+      \<Longrightarrow> \<exists>C. Says A C (Crypt (pubK C) (Nonce NB)) \<in> set evs"
+by (blast intro: B_trusts_NS3_lemma)
+
+
+(*Can we strengthen the secrecy theorem Spy_not_see_NB?  NO*)
+lemma "\<lbrakk>A \<notin> bad;  B \<notin> bad;  evs \<in> ns_public\<rbrakk>            
+       \<Longrightarrow> Says B A (Crypt (pubK A) \<lbrace>Nonce NA, Nonce NB\<rbrace>) \<in> set evs  
+           \<longrightarrow> Nonce NB \<notin> analz (spies evs)"
+apply (erule ns_public.induct, simp_all)
+apply spy_analz
+(*NS1: by freshness*)
+apply (blast)
+(*NS2: by freshness and unicity of NB*)
+apply (blast intro: no_nonce_NS1_NS2)
+(*NS3: unicity of NB identifies A and NA, but not B*)
+apply clarify
+apply (frule_tac A' = "A" in 
+       Says_imp_knows_Spy [THEN parts.Inj, THEN unique_NB])
+apply auto
+apply (rename_tac C B' evs3)
+oops
+
+(*
+THIS IS THE ATTACK!
+Level 8
+!!evs. \<lbrakk>A \<notin> bad; B \<notin> bad; evs \<in> ns_public\<rbrakk>
+       \<Longrightarrow> Says B A (Crypt (pubK A) \<lbrace>Nonce NA, Nonce NB\<rbrace>) \<in> set evs \<longrightarrow>
+           Nonce NB \<notin> analz (spies evs)
+ 1. !!C B' evs3.
+       \<lbrakk>A \<notin> bad; B \<notin> bad; evs3 \<in> ns_public
+        Says A C (Crypt (pubK C) \<lbrace>Nonce NA, Agent A\<rbrace>) \<in> set evs3;
+        Says B' A (Crypt (pubK A) \<lbrace>Nonce NA, Nonce NB\<rbrace>) \<in> set evs3; 
+        C \<in> bad;
+        Says B A (Crypt (pubK A) \<lbrace>Nonce NA, Nonce NB\<rbrace>) \<in> set evs3;
+        Nonce NB \<notin> analz (spies evs3)\<rbrakk>
+       \<Longrightarrow> False
+*)
 
 end
